theories/opsem_systemF_ctx.v
@@ -1,8 +1,11 @@
 Set Warnings "-notation-overridden,-parsing,-deprecated-hint-without-locality".
-From Coq Require Import Relations.Relation_Operators.
-From stdpp Require Import gmap list.
+From stdpp Require Import list relations.
 Require Import Autosubst.Autosubst.
 From logical_relation Require Import syntax_systemF opsem_systemF.
+
+
+(*** Operational semantic of SystemF
+     --- w/ evaluation context *)
 
 Reserved Notation "t '-h->' t'" (at level 60).
 Inductive pure_step : expr -> expr -> Prop :=
@@ -55,11 +58,33 @@ Inductive step e1 e2 : Prop :=
 where "e1 '~>' e2" := (step e1 e2).
 Hint Constructors step : core.
 
-Definition mstep :=  clos_refl_trans_1n expr step.
-Notation "t '~>*' t'" := (mstep t t') (at level 60).
+(** Useful lifting of pure step to step *)
+Lemma step_fst_val v1 v2:
+  is_val v1 ->
+  is_val v2 ->
+  <{ fst (⟨ v1, v2 ⟩) }> ~> v1.
+Proof.
+  intros; eapply (Step _ _ EmptyCtx); eauto.
+Qed.
 
-Lemma fill_empty e : fill EmptyCtx e = e.
-Proof. done. Qed.
+Lemma step_snd_val v1 v2:
+  is_val v1 ->
+  is_val v2 ->
+  <{ snd (⟨ v1, v2 ⟩) }> ~> v2.
+Proof.
+  intros; eapply (Step _ _ EmptyCtx); eauto.
+Qed.
+
+Lemma step_app_val e v:
+  is_val v ->
+  <{ (λ _, e) v }> ~>  e.[v/].
+Proof.
+  intros; eapply (Step _ _ EmptyCtx); eauto.
+Qed.
+#[export] Hint Resolve step_fst_val step_snd_val step_app_val : core.
+
+Definition mstep := rtc step.
+Notation "t '~>*' t'" := (mstep t t') (at level 60).
 
 Lemma is_val_stuck : forall e e', is_val e -> not (e ~> e').
 Proof.
@@ -74,11 +99,11 @@ Proof.
     + eapply IHe1 with (fill K e2') in H1.
       apply H1.
       inversion H3; subst.
-      eapply (Step _ _ K); auto.
+      econstructor; eauto.
     + eapply IHe2 with (fill K e2') in H2.
       apply H2.
       inversion H3; subst.
-      eapply (Step _ _ K); auto.
+      econstructor; eauto.
   - destruct K; subst; simpl in *; try discriminate H3.
     rewrite <- H in H2; inversion H2.
     all:try discriminate H.
@@ -93,6 +118,66 @@ Lemma is_val_step : forall e e', is_val e -> e ~>* e' -> e' = e.
   by apply is_val_stuck in H.
 Qed.
 
+Lemma pure_step_deterministic : forall e e1 e2,
+  e -h-> e1 -> e -h-> e2 -> e1 = e2.
+Proof.
+  intros e e1 e2 step1 step2.
+  induction step1;inversion_clear step2;auto.
+Qed.
+
+(** --- DETERMINISM --- *)
+(* To prove the determinism, we use the determinism of the semantic without
+   evaluation context, and the equivalence between the semantics *)
+Theorem opsem_equivalent:
+  forall e e',
+   opsem_systemF_ctx.step e e' <-> opsem_systemF.step e e'.
+Proof.
+Hint Resolve is_val_of_val : core.
+  intros.
+  split; intros.
+  - induction H.
+    subst.
+    induction K; intros; subst; simpl;
+      try (by inversion H1; subst; auto).
+  - induction H;
+    match goal with
+      | h: _ ~> _ |- ?e1 ~> ?e2 => idtac
+      | h: _ |- ?e1 ~> ?e2 =>
+          eapply (Step _ _ EmptyCtx e1 e2 ); auto
+      end.
+    + inversion IHstep; subst.
+      eapply (Step _ _ (FstCtx K) e1' e2' ); auto.
+    + inversion IHstep; subst.
+      eapply (Step _ _ (SndCtx K) e1' e2' ); auto.
+    + inversion IHstep; subst.
+      eapply (Step _ _ (LPairCtx K _) _ _); auto.
+    + inversion IHstep; subst.
+      apply is_val_inversion in H ; destruct H as [v' Hv]; subst.
+      eapply (Step _ _ (RPairCtx K v') e1' e2'); auto.
+    + inversion IHstep; subst.
+      eapply (Step _ _ (LAppCtx K _) _ _); auto.
+    + inversion IHstep; subst.
+      apply is_val_inversion in H ; destruct H as [v' Hv]; subst.
+      eapply (Step _ _ (RAppCtx K _) e1' e2'); auto.
+    + inversion IHstep; subst.
+      eapply (Step _ _ (TAppCtx K) _ _); auto.
+Qed.
+
+Lemma sf_deterministic : forall e e1 e2, e ~> e1 -> e ~> e2 -> e1 = e2.
+Proof.
+  intros.
+  apply opsem_systemF.sf_deterministic with (e:=e) ; by apply opsem_equivalent.
+Qed.
+
+(** --- ECTX facts --- *)
+
+Lemma fill_K_injective K : forall e e',
+ fill K e = fill K e' -> e = e'.
+Proof.
+  intros.
+  induction K;cbn in *;auto;apply IHK; by injection H.
+Qed.
+
 Fixpoint comp_ectx (K: ectx) (K' : ectx) : ectx :=
   match K with
   | EmptyCtx => K'
@@ -104,50 +189,41 @@ Fixpoint comp_ectx (K: ectx) (K' : ectx) : ectx :=
   | RAppCtx K v => RAppCtx (comp_ectx K K') v
   | TAppCtx K => TAppCtx (comp_ectx K K')
   end.
-
 Lemma fill_comp (K1 K2 : ectx) e : fill K1 (fill K2 e) = fill (comp_ectx K1 K2) e.
 Proof. induction K1; simpl; congruence. Qed.
 
+Lemma fill_empty e : fill EmptyCtx e = e. Proof. done. Qed.
+
 Lemma pure_contextual_step e1 e2 :
-  pure_step e1 e2 → step e1 e2.
-Proof. eapply (Step _ _ EmptyCtx) ; by rewrite ?fill_empty. Qed.
+  e1 -h-> e2 → e1 ~> e2.
+Proof. econstructor;eauto;rewrite fill_empty;reflexivity. Qed.
 
 Lemma fill_contextual_step K e1 e2 :
-  step e1 e2 → step (fill K e1) (fill K e2).
+  e1 ~> e2 → (fill K e1) ~> (fill K e2).
 Proof.
   destruct 1 as [K' e1' e2' -> ->].
   rewrite !fill_comp. by econstructor.
 Qed.
 
-Lemma pure_step_deterministic : forall e e1 e2,
-  e -h-> e1 -> e -h-> e2 -> e1 = e2.
-Proof.
-  intros e e1 e2 step1 step2.
-  induction step1;inversion_clear step2;auto.
-Qed.
-
-Lemma step_fill K : forall e e',
-    e ~> e' ->
-    fill K e ~> fill K e'.
+Lemma step_in_ectx K : forall e e',
+  e ~> e' -> fill K e ~> fill K e'.
 Proof.
   intros.
   inversion H; subst.
   rewrite! fill_comp.
-  eapply Step; eauto.
+  econstructor; eauto.
 Qed.
 
-Lemma mstep_fill K : forall e e',
-  e ~>* e' ->
-  fill K e ~>* fill K e'.
+Lemma mstep_in_ectx K : forall e e',
+  e ~>* e' -> fill K e ~>* fill K e'.
 Proof.
   intros. generalize dependent K.
   induction H; intros.
   + constructor.
-  + apply (step_fill K) in H.
+  + apply (step_in_ectx K) in H.
     econstructor;eauto.
     firstorder.
 Qed.
-
 
 Lemma is_val_fill K e :
   is_val (fill K e) -> is_val e.
@@ -156,50 +232,6 @@ Proof.
   induction K; inversion H; cbn in *; subst;auto.
 Qed.
 
-(* If pure step from (fill K e), then either
-   - e is a value
-   - K is empty
- *)
-Lemma pure_step_fill :
-∀ K e e', (fill K e) -h-> e' → (∀ e'', (fill K e'') = e'') ∨ is_val e.
-Proof.
-  induction K;intros.
-  - (* Empty *)
-    left; cbn in *;intros;auto.
-  - (* Fst *)
-    destruct K; inversion H; subst; right.
-    econstructor; eauto.
-    by eapply is_val_fill.
-    by eapply is_val_fill.
-  - (* Snd *)
-    destruct K; inversion H; subst; right.
-    econstructor; eauto.
-    by eapply is_val_fill.
-    by eapply is_val_fill.
-  - (* PairL *)
-    destruct K; inversion H; subst; right.
-  - (* PairR *)
-    destruct K; inversion H; subst; right.
-  - (* AppL *)
-    destruct K; inversion H; subst; right; constructor.
-  - (* AppR *)
-    inversion H; subst; right.
-    by eapply is_val_fill.
-  - (* TApp *)
-    destruct K; inversion H; subst; right; constructor.
-Qed.
-
-Lemma of_val_injective : forall e1 e2,
-of_val e1 = of_val e2 -> e1 = e2.
-Proof.
-  induction e1; intros; destruct e2;cbn in H; auto; try discriminate;injection H
-  ;intros.
-  - apply IHe1_1 in H1;subst.
-    apply IHe1_2 in H0;subst.
-    reflexivity.
-  - by subst.
-  - by subst.
-Qed.
 
 Lemma ectx_decompose K1 K2 e1 e2 :
   (fill K1 e1) = (fill K2 e2) →
@@ -292,55 +324,38 @@ Proof.
      ;[left|right]; exists K3; intros; by rewrite HeqK.
 Qed.
 
-Lemma fill_K_injective K : forall e e',
- fill K e = fill K e' -> e = e'.
+(* Possible outcomes of a pure step from K[e] *)
+Lemma pure_step_fill :
+∀ K e e', (fill K e) -h-> e' → (∀ e'', (fill K e'') = e'') ∨ is_val e.
 Proof.
-  intros.
-  induction K;cbn in *;auto;apply IHK; by injection H.
+  induction K;intros.
+  - (* Empty *)
+    left; cbn in *;intros;auto.
+  - (* Fst *)
+    destruct K; inversion H; subst; right.
+    econstructor; eauto.
+    by eapply is_val_fill.
+    by eapply is_val_fill.
+  - (* Snd *)
+    destruct K; inversion H; subst; right.
+    econstructor; eauto.
+    by eapply is_val_fill.
+    by eapply is_val_fill.
+  - (* PairL *)
+    destruct K; inversion H; subst; right.
+  - (* PairR *)
+    destruct K; inversion H; subst; right.
+  - (* AppL *)
+    destruct K; inversion H; subst; right; constructor.
+  - (* AppR *)
+    inversion H; subst; right.
+    by eapply is_val_fill.
+  - (* TApp *)
+    destruct K; inversion H; subst; right; constructor.
 Qed.
 
-Theorem opsem_equivalent:
-  forall e e',
-   opsem_systemF_ctx.step e e' <-> opsem_systemF.step e e'.
-Proof.
-Hint Resolve is_val_of_val : core.
-  intros.
-  split; intros.
-  - induction H.
-    subst.
-    induction K; intros; subst; simpl;
-      try (by inversion H1; subst; auto).
-  - induction H;
-    match goal with
-      | h: _ ~> _ |- ?e1 ~> ?e2 => idtac
-      | h: _ |- ?e1 ~> ?e2 =>
-          eapply (Step _ _ EmptyCtx e1 e2 ); auto
-      end.
-    + inversion IHstep; subst.
-      eapply (Step _ _ (FstCtx K) e1' e2' ); auto.
-    + inversion IHstep; subst.
-      eapply (Step _ _ (SndCtx K) e1' e2' ); auto.
-    + inversion IHstep; subst.
-      eapply (Step _ _ (LPairCtx K _) _ _); auto.
-    + inversion IHstep; subst.
-      apply is_val_inversion in H ; destruct H as [v' Hv]; subst.
-      eapply (Step _ _ (RPairCtx K v') e1' e2'); auto.
-    + inversion IHstep; subst.
-      eapply (Step _ _ (LAppCtx K _) _ _); auto.
-    + inversion IHstep; subst.
-      apply is_val_inversion in H ; destruct H as [v' Hv]; subst.
-      eapply (Step _ _ (RAppCtx K _) e1' e2'); auto.
-    + inversion IHstep; subst.
-      eapply (Step _ _ (TAppCtx K) _ _); auto.
-Qed.
-
-Lemma sf_deterministic : forall e e1 e2, e ~> e1 -> e ~> e2 -> e1 = e2.
-Proof.
-  intros.
-  apply opsem_systemF.sf_deterministic with (e:=e) ; by apply opsem_equivalent.
-Qed.
-
-Lemma step_ectx (K : ectx) e e' :
+(* Possible outcomes of a step from K[e] *)
+Lemma step_fill (K : ectx) e e' :
     (fill K e) ~> e' →
     (is_val e) ∨ (∃ e'', e ~> e'' ∧ e' = (fill K e'')).
 Proof.
@@ -372,67 +387,26 @@ Proof.
       eapply Step;eauto.
 Qed.
 
-Inductive nstep : nat → expr → expr → Prop :=
-| no_step e : nstep 0 e e
-| next_step n e1 e2 e3 : step e1 e2 → nstep n e2 e3 → nstep (S n) e1 e3.
-
-Lemma mstep_nstep e e' : mstep e e' → ∃ n, nstep n e e'.
-Proof.
-  intros. induction H as [| ????? IHstar].
-  - exists 0 ; constructor.
-  - destruct IHstar as (n & IH). exists (S n).
-    econstructor;eauto.
-Qed.
-
-Lemma nstep_mstep n e e' : nstep n e e' → mstep e e'.
-Proof.
-  induction 1; econstructor;eauto.
-Qed.
-
-Lemma mstep_ectx (K : ectx) e e' :
+(* Possible outcomes of a mstep from K[e] *)
+Lemma mstep_fill (K : ectx) e e' :
     (fill K e) ~>* e' →
     (∃ e'', e' = (fill K e'') ∧ e ~>* e'')
     ∨ (∃ v , is_val v ∧ e ~>* v ∧ (fill K v) ~>* e').
 Proof.
   intros.
-  apply mstep_nstep in H.
+  apply rtc_nsteps in H.
   destruct H as [n Hnstep].
   revert e e' Hnstep.
   induction n; intros e e' Hnstep.
   - inversion Hnstep; subst; left; exists e ; split; auto; constructor.
   - inversion Hnstep as [|n' e1 e2 e3 HfillK Hnstep2];subst.
-    apply step_ectx in HfillK.
+    apply step_fill in HfillK.
     destruct HfillK as [HfillK | (e'' & Hstep_e & ->)].
     + right; exists e.
       split;auto.
       split;[constructor|].
-      eapply nstep_mstep;eauto.
+      eapply rtc_nsteps_2;eauto.
     + apply IHn in Hnstep2.
       destruct Hnstep2 as [ (e3 &?) | (e3 &?) ]
       ; [left | right]; exists e3; firstorder; econstructor;eauto.
 Qed.
-
-Lemma step_fst_val v1 v2:
-  is_val v1 ->
-  is_val v2 ->
-  <{ fst (⟨ v1, v2 ⟩) }> ~> v1.
-Proof.
-  intros; eapply (Step _ _ EmptyCtx); eauto.
-Qed.
-
-Lemma step_snd_val v1 v2:
-  is_val v1 ->
-  is_val v2 ->
-  <{ snd (⟨ v1, v2 ⟩) }> ~> v2.
-Proof.
-  intros; eapply (Step _ _ EmptyCtx); eauto.
-Qed.
-
-Lemma step_app_val e v:
-  is_val v ->
-  <{ (λ _, e) v }> ~>  e.[v/].
-Proof.
-  intros; eapply (Step _ _ EmptyCtx); eauto.
-Qed.
-
-#[export] Hint Resolve step_fst_val step_snd_val step_app_val : core.
